\documentclass{article}
\usepackage[utf8]{inputenc}
\usepackage[left=2cm, right=2cm, top=2cm, bottom=2cm]{geometry}


\author{Curtis Rau, Colin Gordon, and David Witalka}
\title{A Search Algorithm for Continuous Phase Modulated Gravitational Waves Originating from Binary Neutron Star Systems}

\begin{document}

Last time we took the schrodinger equation and transformed it to the radial equation in center of mass frame.

\begin{equation}
\right[ \left( = \frac{\hbar^2}{m} \frac{1}{r^2} \partial_r r^2 \partial_r + \frac{1}{4} m \omega^2 r^2 + \frac{k e^2}{r} \right)
+ \left( - \frac{\hbar^2}{4m} \frac{1}{R^2} \partial_R R^2 \partial_R + m\omega^2 R^2 + \frac{\hbar l(l+1)}{R^2} \right) \right] \psi (r) \theta (R)  = (E_r + E_R) \psi (r) \theta (R)
\end{equation}

we are only interested in the 

\begin{equation}
\left( = \frac{\hbar^2}{m} \frac{1}{r^2} \partial_r r^2 \partial_r + \frac{1}{4} m \omega^2 r^2 + \frac{k e^2}{r} \right) \psi (r)  = E_r \psi (r)
\end{equation}

we can make the equation dimentionless which gives

\begin{equation}
\left( - \partial_\rho^2 + \rho^2 + \frac{\beta}{\rho} \right) u ( \rho ) = \lambda u(\rho ) \\
\left( - \partial_\rho^2 + V (\rho ) \right) u ( \rho ) = \lambda u(\rho )
\end{equation}

Discretize

\begin{equation}
\begin{aligned}
u(\rho) \to u(\rho_i) = u_i \\
\rho \to \rho_i = \rho_0 + i h \\
h = \frac{b-a}{n+1} \\
a = 0
\end{aligned}
\end{equation}


the linear algebra equation is

\begin{equation}
\hat{A} = 
\left( \begin{array}{cccc}
	 \frac{2}{h^2} + V_1 &    -\frac{1}{h^2}   &                &                        \\
	-\frac{1}{h^2}       & \frac{2}{h^2} + V_2 & -\frac{1}{h^2} &                        \\
	                     &                     &     \ddots     &                        \\
	                     &                     &                &    -\frac{1}{h^2}      \\
	                     &                     & -\frac{1}{h^2} & \frac{2}{h^2} + V_{N-1}
   \end{array} \right)
\end{equation}

\begin{eqnarray}
\hat{A} x = \lambda x \\
S^T A x = \lambda S^T x \\
S^T A S (S^T x) = \lambda (S^T x)
\end{eqnarray}

Eignevalues unchanged under orthogonal transforms

Eigenvectros change, but the length is preserved

Dot product between vectors is conserved

\end{document}